Monads Monads Monads

src/5.1.lean
@@ -33,23 +33,158 @@ Both methods have the correct type. Why does this instance
 violate the monad contract?
 -/
 
---Correct instance
-instance : Monad Option where
-  pure x := some x
-  bind opt next :=
-    match opt with
-    | none => none
-    | some x => next x
+#check Option
+#check Pure
 
-#check Pure.pure
-#check Bind.bind
-#check Monad Option
---#eval pure (some 3 : Option Nat)
+inductive COption (α : Type) : Type
+| none : COption α
+| some : α -> COption α
 
---I can't prove the monad contract :(
-example [Monad m] (f : Option α → m (Option α)) (o : Option α):
-bind (pure o) f = f o := by
-  simp [Monad]
-  sorry
+instance : Monad COption where
+pure arg := COption.some arg
+bind item func := 
+  match item with
+  | COption.none => COption.none
+  | COption.some arg => func arg
 
+--Proof that the default instance of Option satisfies the
+--monad contract
+example (f : α → COption β) (o : α):
+bind (pure o) f = f o := by{
+  rw [pure, Applicative.toPure, Monad.toApplicative,
+   instMonadCOption]
+  simp
+  rw [bind, Monad.toBind]
+}
+
+--Again but using a dedicated Prop so i can prove the
+--2nd part of the problem
+def monadContract (m : Type → Type) (α β : Type) [Monad m] : Prop :=
+∀ (f : α → m β) (o : α), bind (pure o) f = f o 
+
+#check @monadContract
+
+--COption satisfies the monad contract
+example {α β : Type}: monadContract COption α β
+:= by{
+  rw [monadContract, pure, Applicative.toPure,
+      Monad.toApplicative, instMonadCOption]
+  simp
+  rw [bind, Monad.toBind]
+  simp
+}
+
+inductive BOption (α : Type) : Type
+| none : BOption α
+| some : α -> BOption α
+
+instance : Monad BOption where
+pure arg := BOption.some arg
+bind _ _ := BOption.none
+
+#check Exists.intro
+
+--Some random lemmas I was using for this
+
+--This is such a jank proof of this lmao
+theorem L1 (α : Type) (p : α->Prop) :
+(¬∀(x : α),p x) <-> (∃(x : α),¬(p x))
+:= by{
+  rw [Not];
+  apply Iff.intro{
+    intro H;
+    apply Classical.byContradiction;
+    intro H2;
+    rw [Not] at H2;
+    apply H;
+    intro x;
+    apply Classical.byContradiction;
+    intro H3;
+    apply H2;
+    apply Exists.intro x;
+    exact H3;
+  }{
+    intros H1 H2;
+    apply Exists.elim H1;
+    intros x npx;
+    have H3 := H2 x;
+    trivial
+  }
+} 
+
+theorem L2: ∀(p : Prop), ¬¬p <-> p :=
+by{
+  intro p;
+  apply Iff.intro{
+    intro H;
+    rewrite [Not, Not] at H;
+    apply Classical.byContradiction;
+    intros np;
+    apply H;
+    intro;
+    contradiction;
+  }{
+    intro H;
+    rewrite [Not, Not];
+    intro H2;
+    apply H2;
+    exact H;
+  }
+}  
+
+--Proof BOption does not satisfy the monad contract. I'm 
+--only able to prove this so far assuming β and α are nonempty types
+example {α β : Type} [iβ : Nonempty β] [iα : Nonempty α]:
+¬monadContract BOption α β
+:= by{
+  rw [monadContract];
+  rewrite [L1];
+  have b := @Classical.choice β iβ;
+  let f1 := (fun (_ : α) => BOption.some b);
+  apply Exists.intro f1;
+  rewrite [L1];
+  have a := @Classical.choice α iα;
+  apply Exists.intro a;
+  rw [Not]
+  intro H;
+  rw [pure, Applicative.toPure,
+      Monad.toApplicative, instMonadBOption] at H;
+  simp at H;
+}
+
+
+
+--Some scratch work and wrong directions
+
+-- example {α β : Type} [iβ : Nonempty β] [iα : Nonempty α]:
+-- ¬monadContract BOption α β 
+-- := by{
+--   rw [monadContract]
+--   apply @Classical.byContradiction _;
+--   intro H;
+--   rw [L2] at H;
+
+-- }
+
+-- example (f : α → BOption β) (o : α):
+-- bind (pure o) f ≠ f o := by{
+  
+-- }
+
+
+-- example [instB: Nonempty β] (f : α → BOption β) (o : α):
+-- bind (pure o) f = f o := by{
+--   rw [pure, Applicative.toPure, Monad.toApplicative,
+--    instMonadBOption]
+--   simp
+--   rw [bind, Monad.toBind]
+--   simp
+--   --There exists some function for which
+--   --BOption.none ≠ f o
+--   have b : β := @Classical.choice β instB{
+--     have f1 := (fun (a : α) => BOption.some b){
+--       sorry
+--     }
+--   }
+-- }
 
